Weidenbach_Book/IsaSAT_VMTF.thy
@@ -572,10 +572,10 @@ lemma size_conflict_int_size_conflict:
       lookup_clause_rel_def)
 
 definition rescore_clause
-  :: \<open>nat multiset \<Rightarrow> nat clause_l \<Rightarrow> (nat,nat)ann_lits \<Rightarrow> vmtf_remove_int \<Rightarrow> phase_saver \<Rightarrow>
-    (vmtf_remove_int \<times> phase_saver) nres\<close>
+  :: \<open>nat multiset \<Rightarrow> nat clause_l \<Rightarrow> (nat,nat)ann_lits \<Rightarrow> vmtf_remove_int \<Rightarrow>
+    (vmtf_remove_int) nres\<close>
 where
-  \<open>rescore_clause \<A> C M vm \<phi> = SPEC (\<lambda>(vm', \<phi>' :: bool list). vm' \<in> vmtf \<A> M \<and> phase_saving \<A> \<phi>')\<close>
+  \<open>rescore_clause \<A> C M vm = SPEC (\<lambda>(vm'). vm' \<in> vmtf \<A> M)\<close>
 
 (* TODO ded-uplicate definitions *)
 definition find_decomp_w_ns_pre where
@@ -841,81 +841,79 @@ definition find_decomp_wl_st_int :: \<open>nat \<Rightarrow> twl_st_wl_heur \<Ri
 
 
 definition vmtf_rescore_body
- :: \<open>nat multiset \<Rightarrow> nat clause_l \<Rightarrow> (nat,nat) ann_lits \<Rightarrow> vmtf_remove_int \<Rightarrow> phase_saver \<Rightarrow>
-    (nat \<times> vmtf_remove_int \<times> phase_saver) nres\<close>
+ :: \<open>nat multiset \<Rightarrow> nat clause_l \<Rightarrow> (nat,nat) ann_lits \<Rightarrow> vmtf_remove_int \<Rightarrow>
+    (nat \<times> vmtf_remove_int) nres\<close>
 where
-  \<open>vmtf_rescore_body \<A>\<^sub>i\<^sub>n C _ vm \<phi> = do {
-         WHILE\<^sub>T\<^bsup>\<lambda>(i, vm, \<phi>). i \<le> length C  \<and>
-            (\<forall>c \<in> set C. atm_of c < length \<phi> \<and> atm_of c < length (fst (fst vm)))\<^esup>
-           (\<lambda>(i, vm, \<phi>). i < length C)
-           (\<lambda>(i, vm, \<phi>). do {
+  \<open>vmtf_rescore_body \<A>\<^sub>i\<^sub>n C _ vm = do {
+         WHILE\<^sub>T\<^bsup>\<lambda>(i, vm). i \<le> length C  \<and>
+            (\<forall>c \<in> set C. atm_of c < length (fst (fst vm)))\<^esup>
+           (\<lambda>(i, vm). i < length C)
+           (\<lambda>(i, vm). do {
                ASSERT(i < length C);
                ASSERT(atm_of (C!i) \<in># \<A>\<^sub>i\<^sub>n);
                let vm' = vmtf_mark_to_rescore (atm_of (C!i)) vm;
-               RETURN(i+1, vm', \<phi>)
+               RETURN(i+1, vm')
              })
-           (0, vm, \<phi>)
+           (0, vm)
     }\<close>
 
 definition vmtf_rescore
- :: \<open>nat multiset \<Rightarrow> nat clause_l \<Rightarrow> (nat,nat) ann_lits \<Rightarrow> vmtf_remove_int \<Rightarrow> phase_saver \<Rightarrow>
-       (vmtf_remove_int \<times> phase_saver) nres\<close>
+ :: \<open>nat multiset \<Rightarrow> nat clause_l \<Rightarrow> (nat,nat) ann_lits \<Rightarrow> vmtf_remove_int \<Rightarrow>
+       (vmtf_remove_int) nres\<close>
 where
-  \<open>vmtf_rescore \<A>\<^sub>i\<^sub>n C M vm \<phi> = do {
-      (_, vm, \<phi>) \<leftarrow> vmtf_rescore_body \<A>\<^sub>i\<^sub>n C M vm \<phi>;
-      RETURN (vm, \<phi>)
+  \<open>vmtf_rescore \<A>\<^sub>i\<^sub>n C M vm = do {
+      (_, vm) \<leftarrow> vmtf_rescore_body \<A>\<^sub>i\<^sub>n C M vm;
+      RETURN (vm)
    }\<close>
 
 find_theorems isa_vmtf_mark_to_rescore
 
 definition isa_vmtf_rescore_body
- :: \<open>nat clause_l \<Rightarrow> trail_pol \<Rightarrow> isa_vmtf_remove_int \<Rightarrow> phase_saver \<Rightarrow>
-    (nat \<times> isa_vmtf_remove_int \<times> phase_saver) nres\<close>
+ :: \<open>nat clause_l \<Rightarrow> trail_pol \<Rightarrow> isa_vmtf_remove_int \<Rightarrow>
+    (nat \<times> isa_vmtf_remove_int) nres\<close>
 where
-  \<open>isa_vmtf_rescore_body C _ vm \<phi> = do {
-         WHILE\<^sub>T\<^bsup>\<lambda>(i, vm, \<phi>). i \<le> length C  \<and>
-            (\<forall>c \<in> set C. atm_of c < length \<phi> \<and> atm_of c < length (fst (fst vm)))\<^esup>
-           (\<lambda>(i, vm, \<phi>). i < length C)
-           (\<lambda>(i, vm, \<phi>). do {
+  \<open>isa_vmtf_rescore_body C _ vm = do {
+         WHILE\<^sub>T\<^bsup>\<lambda>(i, vm). i \<le> length C  \<and>
+            (\<forall>c \<in> set C. atm_of c < length (fst (fst vm)))\<^esup>
+           (\<lambda>(i, vm). i < length C)
+           (\<lambda>(i, vm). do {
                ASSERT(i < length C);
                ASSERT(isa_vmtf_mark_to_rescore_pre (atm_of (C!i)) vm);
                let vm' = isa_vmtf_mark_to_rescore (atm_of (C!i)) vm;
-               RETURN(i+1, vm', \<phi>)
+               RETURN(i+1, vm')
              })
-           (0, vm, \<phi>)
+           (0, vm)
     }\<close>
 
 definition isa_vmtf_rescore
- :: \<open>nat clause_l \<Rightarrow> trail_pol \<Rightarrow> isa_vmtf_remove_int \<Rightarrow> phase_saver \<Rightarrow>
-       (isa_vmtf_remove_int \<times> phase_saver) nres\<close>
+ :: \<open>nat clause_l \<Rightarrow> trail_pol \<Rightarrow> isa_vmtf_remove_int \<Rightarrow>
+       (isa_vmtf_remove_int) nres\<close>
 where
-  \<open>isa_vmtf_rescore C M vm \<phi> = do {
-      (_, vm, \<phi>) \<leftarrow> isa_vmtf_rescore_body C M vm \<phi>;
-      RETURN (vm, \<phi>)
+  \<open>isa_vmtf_rescore C M vm = do {
+      (_, vm) \<leftarrow> isa_vmtf_rescore_body C M vm;
+      RETURN (vm)
     }\<close>
 
 lemma vmtf_rescore_score_clause:
-  \<open>(uncurry3 (vmtf_rescore \<A>), uncurry3 (rescore_clause \<A>)) \<in>
-     [\<lambda>(((C, M), vm), \<phi>). literals_are_in_\<L>\<^sub>i\<^sub>n \<A> (mset C) \<and> vm \<in> vmtf \<A> M \<and> phase_saving \<A> \<phi>]\<^sub>f
-     (\<langle>Id\<rangle>list_rel \<times>\<^sub>f Id \<times>\<^sub>f Id \<times>\<^sub>f Id) \<rightarrow> \<langle>Id \<times>\<^sub>f Id\<rangle> nres_rel\<close>
+  \<open>(uncurry2 (vmtf_rescore \<A>), uncurry2 (rescore_clause \<A>)) \<in>
+     [\<lambda>((C, M), vm). literals_are_in_\<L>\<^sub>i\<^sub>n \<A> (mset C) \<and> vm \<in> vmtf \<A> M]\<^sub>f
+     (\<langle>Id\<rangle>list_rel \<times>\<^sub>f Id \<times>\<^sub>f Id) \<rightarrow> \<langle>Id\<rangle> nres_rel\<close>
 proof -
-  have H: \<open>vmtf_rescore_body \<A> C M vm \<phi> \<le>
-        SPEC (\<lambda>(n :: nat, vm', \<phi>' :: bool list). phase_saving \<A> \<phi>' \<and> vm' \<in> vmtf \<A> M)\<close>
-    if M: \<open>vm \<in> vmtf \<A> M\<close>\<open>phase_saving \<A> \<phi>\<close> and C: \<open>\<forall>c\<in>set C. atm_of c \<in> atms_of (\<L>\<^sub>a\<^sub>l\<^sub>l \<A>)\<close>
+  have H: \<open>vmtf_rescore_body \<A> C M vm \<le>
+        SPEC (\<lambda>(n :: nat, vm').  vm' \<in> vmtf \<A> M)\<close>
+    if M: \<open>vm \<in> vmtf \<A> M\<close> and C: \<open>\<forall>c\<in>set C. atm_of c \<in> atms_of (\<L>\<^sub>a\<^sub>l\<^sub>l \<A>)\<close>
     for C vm \<phi> M
     unfolding vmtf_rescore_body_def vmtf_mark_to_rescore_def
     apply (refine_vcg WHILEIT_rule_stronger_inv[where R = \<open>measure (\<lambda>(i, _). length C - i)\<close> and
-       I' = \<open>\<lambda>(i, vm', \<phi>'). phase_saving \<A> \<phi>' \<and> vm' \<in> vmtf \<A> M\<close>])
+       I' = \<open>\<lambda>(i, vm'). vm' \<in> vmtf \<A> M\<close>])
     subgoal by auto
     subgoal by auto
     subgoal using C M by (auto simp: vmtf_def phase_saving_def)
     subgoal using C M by auto
     subgoal using M by auto
-    subgoal by auto
     subgoal using C by (auto simp: atms_of_\<L>\<^sub>a\<^sub>l\<^sub>l_\<A>\<^sub>i\<^sub>n)
-    subgoal using C unfolding phase_saving_def by auto
-    subgoal unfolding phase_saving_def by auto
-    subgoal using C unfolding phase_saving_def by auto
+    subgoal using C by auto
+    subgoal using C by auto
     subgoal using C by (auto simp: vmtf_append_remove_iff')
     subgoal by auto
     done
@@ -937,8 +935,8 @@ proof -
 qed
 
 lemma isa_vmtf_rescore_body:
-  \<open>(uncurry3 (isa_vmtf_rescore_body), uncurry3 (vmtf_rescore_body \<A>)) \<in> [\<lambda>_. isasat_input_bounded \<A>]\<^sub>f
-     (Id \<times>\<^sub>f trail_pol \<A> \<times>\<^sub>f (Id \<times>\<^sub>f distinct_atoms_rel \<A>) \<times>\<^sub>f Id) \<rightarrow> \<langle>Id \<times>\<^sub>r (Id \<times>\<^sub>f distinct_atoms_rel \<A>) \<times>\<^sub>r Id\<rangle> nres_rel\<close>
+  \<open>(uncurry2 (isa_vmtf_rescore_body), uncurry2 (vmtf_rescore_body \<A>)) \<in> [\<lambda>_. isasat_input_bounded \<A>]\<^sub>f
+     (Id \<times>\<^sub>f trail_pol \<A> \<times>\<^sub>f (Id \<times>\<^sub>f distinct_atoms_rel \<A>)) \<rightarrow> \<langle>Id \<times>\<^sub>r (Id \<times>\<^sub>f distinct_atoms_rel \<A>)\<rangle> nres_rel\<close>
 proof -
   show ?thesis
     unfolding isa_vmtf_rescore_body_def vmtf_rescore_body_def uncurry_def
@@ -946,13 +944,13 @@ proof -
     apply refine_rcg
     subgoal by auto
     subgoal by auto
-    subgoal for x y x1 x1a x1b x2 x2a x2b x1c x1d x1e x2c x2d x2e xa x' x1f x2f x1g x2g
-      by (cases x1g) auto
+    subgoal for x y x1 x1a x1b x2 x2a x2b x1c x1d x1e x2c x1g x2g
+      by (cases x2g) auto
     subgoal by auto
     subgoal by auto
-    subgoal for x y x1 x1a x1b x2 x2a x2b x1c x1d x1e x2c x2d x2e xa x' x1f x2f x1g x2g
+    subgoal for x y x1 x1a x1b x2 x2a x2b x1c x1d x1e x2c x2d x2e x1g x2g
       unfolding isa_vmtf_mark_to_rescore_pre_def
-      by (cases x1g)
+      by (cases x2e)
         (auto intro!: atms_hash_insert_pre)
     subgoal
       by (auto intro!:  isa_vmtf_mark_to_rescore_vmtf_mark_to_rescore[THEN fref_to_Down_unRET_uncurry])
@@ -960,13 +958,13 @@ proof -
 qed
 
 lemma isa_vmtf_rescore:
-  \<open>(uncurry3 (isa_vmtf_rescore), uncurry3 (vmtf_rescore \<A>)) \<in> [\<lambda>_. isasat_input_bounded \<A>]\<^sub>f
-     (Id \<times>\<^sub>f trail_pol \<A> \<times>\<^sub>f (Id \<times>\<^sub>f distinct_atoms_rel \<A>) \<times>\<^sub>f Id) \<rightarrow> \<langle>(Id \<times>\<^sub>f distinct_atoms_rel \<A>) \<times>\<^sub>f Id\<rangle> nres_rel\<close>
+  \<open>(uncurry2 (isa_vmtf_rescore), uncurry2 (vmtf_rescore \<A>)) \<in> [\<lambda>_. isasat_input_bounded \<A>]\<^sub>f
+     (Id \<times>\<^sub>f trail_pol \<A> \<times>\<^sub>f (Id \<times>\<^sub>f distinct_atoms_rel \<A>)) \<rightarrow> \<langle>(Id \<times>\<^sub>f distinct_atoms_rel \<A>)\<rangle> nres_rel\<close>
 proof -
   show ?thesis
     unfolding isa_vmtf_rescore_def vmtf_rescore_def uncurry_def
     apply (intro frefI nres_relI)
-    apply (refine_rcg isa_vmtf_rescore_body[THEN fref_to_Down_curry3])
+    apply (refine_rcg isa_vmtf_rescore_body[THEN fref_to_Down_curry2])
     subgoal by auto
     subgoal by auto
     done
